code/AppearsInTree.v
@@ -28,9 +28,93 @@ Proof.
       apply beq_nat_false in Heqb0. omega.
 Qed.
 
+Lemma appears_in_tree_when_appears_in_subtree: forall (X: Type) (b k k1 k2: nat) (t1 t2: bplustree b X) (l1 l2: list (nat * bplustree b X)),
+  appears_in_tree k t1 -> 
+  k1 <= k < k2 ->
+  kvl_sorted (l1 ++ (k1, t1) :: (k2, t2)::l2) ->
+  appears_in_tree k (bptNode b X (l1 ++ (k1, t1) :: (k2, t2)::l2)).
+Proof.
+  intros.
+  induction l1.
+  Case "l1 = []".
+    simpl.
+   apply ait_node_here; assumption.
+     destruct a. rewrite <- app_comm_cons.
+     destruct l1. 
+       simpl.
+       apply ait_node_later. apply IHl1. 
+         simpl. simpl in H1. apply list_tail_is_sorted in H1. apply H1.
+         omega.
+       rewrite <- app_comm_cons. destruct p.
+       destruct l1.
+         simpl. apply ait_node_later. simpl in IHl1. apply IHl1. 
+           simpl in H1. apply list_tail_is_sorted in H1. apply H1.
+           simpl in H1. inversion H1. inversion H4.
+           apply blt_nat_true in H15. omega.
+           
+         rewrite <- app_comm_cons. destruct p.
+         apply ait_node_later. apply IHl1.
+           apply list_tail_is_sorted in H1. apply H1.
+           simpl in H1.
+           inversion H1.
+           apply kvl_sorted_key_across_app with (l1 := ((n1,b2)::l1)) in H4.
+           omega.
+Qed.
+
+Lemma appears_in_tree_when_appears_in_last_subtree: forall (X: Type) (b k k1 k2: nat) (t1 t2: bplustree b X) (l1 l2: list (nat * bplustree b X)),
+  appears_in_tree k t1 -> 
+  k1 <= k ->
+  kvl_sorted ((k2,t2)::l1 ++ [(k1, t1)]) ->
+  appears_in_tree k (bptNode b X ((k2,t2)::l1 ++ [(k1, t1)])).
+Proof.
+  intros. generalize dependent k2. generalize dependent t2.
+  induction l1.
+  Case "l1 = []".
+    intros.
+    simpl.
+    apply ait_node_last; assumption.
+  Case "l1 = a::l1". destruct a.
+    intros.
+    destruct l1.
+      simpl.
+      apply ait_node_later. apply ait_node_last; assumption.
+      simpl in H1.
+      inversion H1. inversion H4.
+      apply blt_nat_true in H15. omega.
+      destruct p.
+      repeat rewrite <- app_comm_cons.
+      apply ait_node_later.
+      apply IHl1.
+      simpl in H1. simpl. apply list_tail_is_sorted in H1. apply H1.
+      
+      simpl in H1. apply list_tail_is_sorted in H1.
+      apply kvl_sorted_key_across_app with (l1 := ((n0, b1)::l1)) in H1.
+      omega.
+Qed.    
   
+(*
+Lemma key_valid_when_appears_and_between : forall (X: Type) (b k1 k2 sk: nat) (t: bplustree b X), 
+  appears_in_tree sk t ->
+  all_keys X (between k1 k2) (inorder t)
+  -> k1 <= sk < k2.
+Proof.
+  admit.
+Admitted.
   
-  
-  
-  
+Lemma appears_in_valid_tree_when_appears_in_subtree : forall (X: Type) (b k sk: nat) (t: bplustree b X) (l1 l2: list (nat * bplustree b X)), 
+  valid_bplustree b X (bptNode b X (l1++(k,t)::l2)) ->
+  appears_in_tree sk t ->
+  appears_in_tree sk (bptNode b X (l1++(k,t)::l2)).
+Proof.
+  intros.
+  inversion H.
+  induction l1.
+    simpl in *.
+    inversion H8.
+    apply ait_node_here; try assumption.
+    eapply key_valid_when_appears_and_between.
+      apply H0.
+      apply H11.
+    admit.
+*) 
   
